theories/Izf.v
@@ -1,0 +1,116 @@
+Require Import Blech.Spec.
+Require Import Blech.SpecNotations.
+Require Import Blech.Environment.
+Require Import Blech.Category.
+Require Import Blech.Term.
+Require Import Blech.Context.
+
+Require Import Coq.Unicode.Utf8.
+Require Import Coq.Classes.SetoidClass.
+Require Import Coq.Arith.PeanoNat.
+Require Coq.Lists.List.
+
+Import List.ListNotations.
+Import IfNotations.
+
+Implicit Type Γ: environment.
+Implicit Type Δ: usage.
+Implicit Type E: context.
+Implicit Type t: type.
+Implicit Types x y: var.
+Implicit Type ρ: subst.
+Implicit Type v: intro.
+
+Definition set_x: var := 0.
+Definition set := t_var set_x.
+
+Definition empty_ax: var := 0.
+Definition pair_ax: var := 1.
+Definition union_ax: var := 2.
+Definition infinity_ax: var := 3.
+Definition powerset_ax: var := 4.
+
+(* FIXME allow axiomizing maps *)
+Axiom mem: context → context.
+Notation "∈" := mem.
+
+Axiom mem_use: ∀ {Δ1 Δ2 E},
+    Δ1 ⊢ E ⊠ Δ2 →
+    Δ1 ⊢ ∈ E ⊠ Δ2.
+Axiom mem_check: ∀ {Γ E},
+  check Γ E set →
+  check Γ (∈ E) set.
+
+Definition empty := v_axiom empty_ax t_unit set_x v_tt.
+Notation "∅" := empty.
+
+Definition pair v v' := v_axiom pair_ax (set * set) set_x (v_fanout v v').
+
+Definition union := v_axiom union_ax set set_x.
+Notation "⋃" := union.
+
+Definition infinity := v_axiom infinity_ax t_unit set_x v_tt.
+Notation "∞" := infinity.
+
+Definition powerset := v_axiom powerset_ax set set_x.
+
+Lemma empty_check: ∀ {Γ}, Γ ⊢ ∅ ⇐ set.
+Proof.
+  intro.
+  constructor.
+  constructor.
+Qed.
+
+Lemma pair_check: ∀ {Γ v v'},
+    Γ ⊢ v ⇐ set →
+    Γ ⊢ v' ⇐ set →
+    Γ ⊢ pair v v' ⇐ set.
+Proof.
+  intros.
+  constructor.
+  constructor.
+  all: auto.
+Qed.
+
+Lemma union_check: ∀ {Γ v},
+    Γ ⊢ v ⇐ set →
+    Γ ⊢ ⋃ v ⇐ set.
+Proof.
+  intros.
+  constructor.
+  auto.
+Qed.
+
+Lemma infinity_check: ∀ {Γ},
+    Γ ⊢ ∞ ⇐ set.
+Proof.
+  intros.
+  constructor.
+  constructor.
+Qed.
+
+Lemma powerset_check: ∀ {Γ v},
+    Γ ⊢ v ⇐ set →
+    Γ ⊢ powerset v ⇐ set.
+Proof.
+  intros.
+  constructor.
+  auto.
+Qed.
+
+(* not sure here *)
+Axiom empty_accepts:
+  ∀ {ρ1 ρ2 ρ3 E v},
+    accepts ρ1 E v ρ2 →
+    accepts ρ2 (∈ E) ∅ ρ3 →
+    False.
+    (* accepts ρ2 false v' ρ3. *)
+
+Axiom pair_accepts_1:
+  ∀ {ρ1 ρ2 E v v'},
+    accepts ρ1 E v ρ2 →
+    accepts ρ1 (∈ E) (pair v v') ρ2.
+Axiom pair_accepts_2:
+  ∀ {ρ1 ρ2 E v v'},
+    accepts ρ1 E v' ρ2 →
+    accepts ρ1 (∈ E) (pair v v') ρ2.
